tests/demo/A_o.v
@@ -6,23 +6,26 @@
 From Cpp Require Import
      Auto.
 Require Import Cpp.Sem.Linking.
-From ChargeCore.Logics Require Import
-     ILogic BILogic ILEmbed Later.
 
 From Demo Require
      A_hpp A_hpp_spec A_hpp_proof
      A_cpp A_cpp_spec A_cpp_proof.
 Import A_hpp_spec.
 
+Section with_Σ.
+Context {Σ:gFunctors}.
+
 Theorem A_o_sound (resolve : _)
-: denoteModule A_cpp.module
+: denoteModule (Σ:=Σ) A_cpp.module
   |-- (ti_cglob (resolve:=resolve) A__foo A__foo_spec) **
       (ti_cglob (resolve:=resolve) A__bar A__bar_spec).
 Proof.
-  use_module (A_hpp_proof.A_hpp_sound resolve).
-  use_module (A_cpp_proof.A_cpp_sound resolve).
+  use_module (A_hpp_proof.A_hpp_sound (Σ:=Σ) resolve).
+  use_module (A_cpp_proof.A_cpp_sound (Σ:=Σ) resolve).
   rewrite denoteModule_weaken.
   unfold A_cpp_spec.A_cpp_spec.
   unfold A_hpp_spec.A_hpp_spec.
   module_cancel.
 Qed.
+
+End with_Σ.
