theories/Sem/Call.v
@@ -18,20 +18,24 @@ From Cpp.Sem Require Import
 Module Type Call.
 
   Section with_resolve.
+    Context {Σ:gFunctors}.
     Context {resolve : genv}.
     Variable ti : thread_info.
     Variable ρ : region.
 
-    Local Notation wp := (wp (resolve:=resolve)  ti ρ).
-    Local Notation wpe := (wpe (resolve:=resolve) ti ρ).
-    Local Notation wp_lval := (wp_lval (resolve:=resolve) ti ρ).
-    Local Notation wp_rval := (wp_rval (resolve:=resolve) ti ρ).
-    Local Notation wp_prval := (wp_prval (resolve:=resolve) ti ρ).
-    Local Notation wp_xval := (wp_xval (resolve:=resolve) ti ρ).
-    Local Notation wp_init := (wp_init (resolve:=resolve) ti ρ).
-    Local Notation wpAny := (wpAny (resolve:=resolve) ti ρ).
-    Local Notation wpAnys := (wpAnys (resolve:=resolve) ti ρ).
-    Local Notation fspec := (fspec (resolve:=resolve)).
+    Local Notation wp := (wp (Σ:=Σ) (resolve:=resolve)  ti ρ).
+    Local Notation wpe := (wpe (Σ:=Σ) (resolve:=resolve) ti ρ).
+    Local Notation wp_lval := (wp_lval (Σ:=Σ) (resolve:=resolve) ti ρ).
+    Local Notation wp_rval := (wp_rval (Σ:=Σ) (resolve:=resolve) ti ρ).
+    Local Notation wp_prval := (wp_prval (Σ:=Σ) (resolve:=resolve) ti ρ).
+    Local Notation wp_xval := (wp_xval (Σ:=Σ) (resolve:=resolve) ti ρ).
+    Local Notation wp_init := (wp_init (Σ:=Σ) (resolve:=resolve) ti ρ).
+    Local Notation wpAny := (wpAny (Σ:=Σ) (resolve:=resolve) ti ρ).
+    Local Notation wpAnys := (wpAnys (Σ:=Σ) (resolve:=resolve) ti ρ).
+    Local Notation fspec := (fspec (Σ:=Σ) (resolve:=resolve)).
+
+    Local Notation mpred := (mpred Σ) (only parsing).
+    Local Notation FreeTemps := (FreeTemps Σ) (only parsing).
 
     Fixpoint wp_args (es : list (ValCat * Expr)) (Q : list val -> FreeTemps -> mpred) : mpred :=
       match es with
