theories/Sem/IrisBridge.v
@@ -1,0 +1,80 @@
+From iris Require Import bi.notation.
+From iris Require Import bi.bi.
+
+Global Notation lentails := (bi_entails) (only parsing).
+Global Notation lequiv := (bi_equiv _) (only parsing).
+Global Notation ltrue := (bi_pure True) (only parsing).
+Global Notation lfalse := (bi_pure False) (only parsing).
+Global Notation land := (bi_and) (only parsing).
+Global Notation lor := (bi_or) (only parsing).
+Global Notation limpl := (bi_impl) (only parsing).
+Global Notation lforall := (bi_forall) (only parsing).
+Global Notation lexists := (bi_exist) (only parsing).
+
+Global Notation empSP := (bi_emp) (only parsing).
+Global Notation sepSP := (bi_sep) (only parsing).
+Global Notation wandSP := (bi_wand) (only parsing).
+Global Notation illater := (sbi_later) (only parsing).
+
+Global Notation embed := (bi_pure) (only parsing).
+Ltac split' := intros; apply (anti_symm (⊢)).
+
+Definition only_provable_def {PROP:bi} (P : Prop) :=
+  ((embed (PROP:=PROP) P) ∧ (empSP%I:PROP))%I.
+Definition only_provable_aux : seal (@only_provable_def). by eexists. Qed.
+Definition only_provable := only_provable_aux.(unseal).
+Definition only_provable_eq : @only_provable = _ := only_provable_aux.(seal_eq).
+
+Arguments only_provable {_} _.
+
+(* Charge notation levels *)
+Module ChargeNotation.
+
+  Infix "|--"  := (⊢)%I (at level 80, no associativity).
+  Notation "P //\\ Q"   := (P ∧ Q)%I (at level 75, right associativity).
+  Notation "P \\// Q"   := (P ∨ Q)%I (at level 76, right associativity).
+  Notation "P -->> Q"   := (P → Q)%I (at level 77, right associativity).
+  Notation "'Forall' x .. y , p" :=
+    (lforall (fun x => .. (lforall (fun y => p)) ..))%I (at level 78, x binder, y binder, right associativity).
+
+  Notation "'Exists' x .. y , p" :=
+    (lexists (fun x => .. (lexists (fun y => p)) ..))%I (at level 78, x binder, y binder, right associativity).
+
+  Notation "|--  P" := (bi_pure True |-- P) (at level 85, no associativity).
+
+  Notation "P ** Q" := (P ∗ Q)%I (at level 58, right associativity).
+  Notation "P -* Q" := (P -∗ Q)%I (at level 60, right associativity).
+  Notation "'sepSPs' ps" := ([∗] ps)%I (at level 20).
+
+  Notation "'|>' P" := (▷  P)%I (at level 71).
+
+  Infix "-|-"  := (⊣⊢)%I (at level 85, no associativity).
+  Global Arguments only_provable : simpl never.
+  Notation "'[|'  P  '|]'" := (only_provable P).
+
+End ChargeNotation.
+
+(* IPM notation levels *)
+Module IPMNotation.
+  Notation "P |-- Q" := (P ⊢ Q)%I (at level 99, Q at level 200, right associativity).
+  Notation "P //\\ Q" := (P ∧ Q)%I (at level 99, Q at level 80, right associativity).
+  Notation "P \\// Q" := (P ∨ Q)%I (at level 99, Q at level 85, right associativity).
+  Notation "P -->> Q" := (P → Q)%I (at level 99, Q at level 200, right associativity).
+
+  Notation "'Forall' x .. y , p" :=
+    (lforall (fun x => .. (lforall (fun y => p)) ..))%I (at level 78, x binder, y binder, right associativity).
+  Notation "'Exists' x .. y , p" :=
+    (lexists (fun x => .. (lexists (fun y => p)) ..))%I (at level 78, x binder, y binder, right associativity).
+
+  Infix "-|-"  := (⊣⊢)%I (at level 95, no associativity).
+  Notation "|--  P" := (True |-- P)%I (at level 85, no associativity).
+
+  Notation "P ** Q" := (P ∗ Q)%I (at level 80, right associativity).
+  Notation "P -* Q" := (P -∗ Q)%I (at level 99, Q at level 200, right associativity,
+                                   format "'[' P  '/' -*  Q ']'").
+  Notation "[| P |]" := (⌜ P ⌝%I) (at level 1, P at level 200).
+  Notation "[|| P ||]" := (⎡ P ⎤%I) (at level 1, P at level 200).
+  Notation "'sepSPs' ps" := ([∗] ps)%I (at level 20).
+
+  Notation "|> P" := (▷  P)%I (at level 20, right associativity).
+End IPMNotation.
